ABD/ABD3/Views/All.lean
@@ -12,3 +12,4 @@ import ABD.ABD3.Views.DPlusGraph.All
 import ABD.ABD3.Views.CollisionFrontier
 import ABD.ABD3.Views.CollisionFrontierA
 import ABD.ABD3.Views.CollisionFrontierA2
+import ABD.ABD3.Views.CollisionFrontierPureTwo2.All
