ABD/ABD3/Views/DPlusGraph/All.lean
@@ -1,4 +1,5 @@
 import ABD.ABD3.Views.DPlusGraph.CPort
+import ABD.ABD3.Views.DPlusGraph.LocalSurplus
 import ABD.ABD3.Views.DPlusGraph.Absorption
 import ABD.ABD3.Views.DPlusGraph.Frontier
 import ABD.ABD3.Views.DPlusGraph.Generators
